Add port clearing during tag advancement step

src/ReactorModel/Execution/Reactor.lean
@@ -30,6 +30,24 @@ namespace Proper
 
 variable [Proper α] 
 
+structure Cleared (rtr₁ rtr₂ : α) : Prop where
+  equiv    : rtr₁ ≈ rtr₂
+  eq_state : rtr₁[.stv] = rtr₂[.stv]
+  eq_acts  : rtr₁[.act] = rtr₂[.act]
+  inputs   : ∀ {i v}, rtr₂[.inp][i] = some v → v = .absent  
+  outputs  : ∀ {i v}, rtr₂[.out][i] = some v → v = .absent
+
+theorem Cleared.deterministic {rtr : α} (cl₁ : Cleared rtr rtr₁) (cl₂ : Cleared rtr rtr₂) : 
+    rtr₁ = rtr₂ := by
+  have e := Equivalent.trans (Equivalent.symm cl₁.equiv) cl₂.equiv
+  apply ext_obj? e
+  intro cpt _ _ _ ho₁ ho₂
+  cases cpt
+  case stv => simp_all [(ho₁ ▸ cl₁.eq_state) ▸ (ho₂ ▸ cl₂.eq_state)] 
+  case act => simp_all [(ho₁ ▸ cl₁.eq_acts) ▸ (ho₂ ▸ cl₂.eq_acts)] 
+  case inp => simp [cl₁.inputs ho₁, cl₂.inputs ho₂]
+  case out => simp [cl₁.outputs ho₁, cl₂.outputs ho₂]
+
 -- TODO: Why do we explcitly have to write the `Updatable` here?
 def apply (rtr : α) : Change → α 
   | .inp i v   => Updatable.update rtr .inp i (fun _ => v)
